rope.md
@@ -7,16 +7,38 @@
 3. The root has at least two children if it is not a leaf node.
 4. MIN_LEAF MAX LEAF: maximum value length in leaf
 5. All leaves appear in the same level. (so it seems...)
+  * todo: Height function => height of all children must be identical? [todo]
 6. Only leaves contain data
+  * already ensured by the data structure itself
 7. Weight values (left subtrees)
 
 
 
-# Operations
+## Operations
 
 * Index
+  * not really necessary, but should be easy to implement
+
 * Concat
+  * yes
+
 * Split
+  * Copy?
+
 * Insert
+  * yes
+
 * Delete
+  * does not exists
+    * every time some delta is applied to the text, the `text` rope gets rebuilt from scratch by performing copy and insertion operations
+      * (which is probably faster than deletion)
+
 * Report (output the string)
+  * never the case that entire tree is converted to string
+  * instead only segments of the tree converted into string (eg. only visible parts)
+  * slice_to_cow
+
+
+## Future
+
+* deltas?
